inversion/c/montgomery_jump/secp256k1_64_test.c
@@ -1,0 +1,2 @@
+#include "secp256k1_64.c"
+#include "test_template.c"
