inversion/c/solinas_jump/curve25519_32.c
@@ -1,0 +1,9 @@
+#include "../../../fiat-c/src/curve25519_32.c"
+
+#define LIMBS 10 /* amount of limbs pr. large integer in montgomery domain, see montgomery_inversion */
+#define WORD uint32_t
+#define WORDSIZE 32 /* wordsize */
+#define LEN_PRIME 255 /* length of the prime in bits */
+#define CURVE_DESCRIPTION fiat_25519
+
+#include "template.c"
