inversion/c/solinas_jump/curve25519_32_test.c
@@ -1,0 +1,2 @@
+#include "curve25519_32.c"
+#include "test_template.c"
