inversion/c/solinas_jump_hd/poly1305_64_test.c
@@ -1,0 +1,2 @@
+#include "poly1305_64.c"
+#include "test_template.c"
