inversion/c/solinas_test_template.c
@@ -1,0 +1,132 @@
+#include <stdio.h>
+#include <stdlib.h>
+#include <string.h>
+#include <inttypes.h>
+#include <time.h>
+
+#define MAKE_FN_NAME1(x,y) x ## y
+#define MAKE_FN_NAME(x,y) MAKE_FN_NAME1(x,y)
+
+#define SAT_FROM_BYTES MAKE_FN_NAME(CURVE_DESCRIPTION,_sat_from_bytes)
+#define FROM_BYTES MAKE_FN_NAME(CURVE_DESCRIPTION,_from_bytes)
+#define TO_BYTES MAKE_FN_NAME(CURVE_DESCRIPTION,_to_bytes)
+
+inline long long cpucycles(void) {
+  unsigned long long result;
+  asm volatile(".byte 15;.byte 49;shlq $32,%%rdx;orq %%rdx,%%rax"
+    : "=a" (result) ::  "%rdx");
+  return result;
+}
+
+long long t[64];
+WORD x[SAT_LIMBS];
+
+void bench(void (*inv)(WORD out[LIMBS], WORD in[LIMBS])) {
+  long long i,j;
+  
+  for (i = 0;i < 64;++i)
+    t[i] = cpucycles();
+  for (i = 63;i > 0;--i)
+    t[i] -= t[i-1];
+
+  printf("nothing");
+  for (i = 1;i < 64;++i)
+    printf(" %lld",t[i]);
+  printf("\n");
+
+  for (i = 0;i < 64;++i) {
+    t[i] = cpucycles();
+    inv(x,x);
+  }
+  for (i = 63;i > 0;--i)
+    t[i] -= t[i-1];
+
+  printf("cycles");
+  for (i = 1;i < 64;++i)
+    printf(" %lld",t[i]);
+  printf("\n");
+
+  for (i = 1;i < 64;++i)
+    for (j = 1;j < i;++j)
+      if (t[i] < t[j]) {
+        long long ti = t[i];
+        t[i] = t[j];
+        t[j] = ti;
+      }
+  printf("sorted");
+  for (i = 1;i < 64;++i)
+    printf(" %lld",t[i]);
+  printf("\n");
+  printf("median");
+  printf(" %lld\n",t[32]);
+  
+  fflush(stdout);
+}
+
+int main() {
+  WORD res[LIMBS], out[LIMBS], g[SAT_LIMBS], g1[LIMBS];
+  uint8_t a[BYTES];
+
+  int seed = time(0);
+  srand(seed);
+  printf("seed: %i\n", seed);	
+	
+  for (int j = 0; j < 10000; j++) {
+    int i;
+    for (i = 0; i < BYTES; i++) {
+      a[i] = rand() % 256;
+      if (i > BYTES - 8) a[i] = 0;
+    }
+		
+    SAT_FROM_BYTES(g,a);
+    FROM_BYTES(g1,a);
+	
+    inverse(out,g);
+
+    MUL(res,out,g1);
+    TO_BYTES(a,res);
+		
+    if (a[0] != 1) {
+			/* printf("%" PRIu8 " ", a[0]); */
+      printf("FAIL\n");
+      return 2;
+    }
+    for (i = 1; i < BYTES; i++) {
+      if (a[i] != 0) {
+				/* printf("%" PRIu8 " ", a[i]); */
+        printf("FAIL\n");
+        return 1;
+      }
+    }
+
+#ifdef FLT_INVERSION
+    flt_inverse(out, g1);
+
+    MUL(res,out,g1);
+    TO_BYTES(a,res);
+		
+    if (a[0] != 1) {
+      printf("FAIL\n");
+      return 2;
+    }
+    for (i = 1; i < BYTES; i++) {
+      if (a[i] != 0) {
+        printf("FAIL\n");
+        return 1;
+      }
+    }
+#endif
+		
+  }
+  printf("PASS\n");
+  
+  printf("\nbenchmarking inverse...\n");
+  bench(inverse);
+
+#ifdef FLT_INVERSION
+  printf("\nbenchmarking flt_inverse...\n");
+  bench(flt_inverse);
+#endif 
+  
+  return 0;
+}
