src/PushButtonSynthesis/BYInversionReificationCache.v
@@ -8,7 +8,7 @@ Require Import Crypto.Arithmetic.Partition.
 Require Import Crypto.Arithmetic.Freeze.
 Require Import Crypto.Arithmetic.ModOps.
 Require Import Crypto.Arithmetic.WordByWordMontgomery.
-Require Import Crypto.Arithmetic.BYInv.
+Require Import Crypto.Arithmetic.BYInv.Definitions.
 Require Import Rewriter.Language.Language.
 Require Import Crypto.Language.API.
 Require Import Crypto.PushButtonSynthesis.ReificationCache.
@@ -27,10 +27,89 @@ Import Associational Positional.
 
 Local Set Keyed Unification. (* needed for making [autorewrite] fast, c.f. COQBUG(https://github.com/coq/coq/issues/9283) *)
 
-Module Export WordByWordMontgomeryInversion.
+Definition partition bitwidth n a := Partition.partition (uweight bitwidth) n a. (* similar to encode except it does not inject into Montgomery domain *)
+
+Derive reified_partition_gen
+       SuchThat (is_reification_of reified_partition_gen partition)
+       As reified_partition_gen_correct.
+Proof.
+  Time cache_reify ().
+  Time Qed.
+Hint Extern 1 (_ = _) => apply_cached_reification partition (proj1 reified_partition_gen_correct) : reify_cache_gen.
+Hint Immediate (proj2 reified_partition_gen_correct) : wf_gen_cache.
+Hint Rewrite (proj1 reified_partition_gen_correct) : interp_gen_cache.
+Local Opaque reified_partition_gen. (* needed for making [autorewrite] not take a very long time *)
+
+Derive reified_eval_twos_complement_gen
+         SuchThat (is_reification_of reified_eval_twos_complement_gen tc_eval)
+         As reified_eval_twos_complement_gen_correct.
+  Proof. Time cache_reify (). Time Qed.
+  Hint Extern 1 (_ = _) => apply_cached_reification tc_eval (proj1 reified_eval_twos_complement_gen_correct) : reify_cache_gen.
+  Hint Immediate (proj2 reified_eval_twos_complement_gen_correct) : wf_gen_cache.
+  Hint Rewrite (proj1 reified_eval_twos_complement_gen_correct) : interp_gen_cache.
+  Local Opaque reified_eval_twos_complement_gen. (* needed for making [autorewrite] not take a very long time *)
+
+Module Export WordByWordMontgomery.
+  Import Definitions.WordByWordMontgomery.
   Import WordByWordMontgomery.WordByWordMontgomery.
 
-  Definition msat bitwidth n m := Partition.partition (uweight bitwidth) n m. (* m in saturated representation *)
+  Derive reified_update_fg_gen
+         SuchThat (is_reification_of reified_update_fg_gen update_fg)
+         As reified_update_fg_gen_correct.
+  Proof. Time cache_reify (). Time Qed.
+  Hint Extern 1 (_ = _) => apply_cached_reification update_fg (proj1 reified_update_fg_gen_correct) : reify_cache_gen.
+  Hint Immediate (proj2 reified_update_fg_gen_correct) : wf_gen_cache.
+  Hint Rewrite (proj1 reified_update_fg_gen_correct) : interp_gen_cache.
+  Local Opaque reified_update_fg_gen. (* needed for making [autorewrite] not take a very long time *)
+
+  Derive reified_update_vr_gen
+         SuchThat (is_reification_of reified_update_vr_gen update_vr)
+         As reified_update_vr_gen_correct.
+  Proof. Time cache_reify (). Time Qed.
+  Hint Extern 1 (_ = _) => apply_cached_reification update_vr (proj1 reified_update_vr_gen_correct) : reify_cache_gen.
+  Hint Immediate (proj2 reified_update_vr_gen_correct) : wf_gen_cache.
+  Hint Rewrite (proj1 reified_update_vr_gen_correct) : interp_gen_cache.
+  Local Opaque reified_update_vr_gen. (* needed for making [autorewrite] not take a very long time *)
+
+  Derive reified_inner_loop_gen
+         SuchThat (is_reification_of reified_inner_loop_gen inner_loop)
+         As reified_inner_loop_gen_correct.
+  Proof. Time cache_reify (). Time Qed.
+  Hint Extern 1 (_ = _) => apply_cached_reification inner_loop (proj1 reified_inner_loop_gen_correct) : reify_cache_gen.
+  Hint Immediate (proj2 reified_inner_loop_gen_correct) : wf_gen_cache.
+  Hint Rewrite (proj1 reified_inner_loop_gen_correct) : interp_gen_cache.
+  Local Opaque reified_inner_loop_gen. (* needed for making [autorewrite] not take a very long time *)
+
+  Derive reified_inner_loop_hd_gen
+         SuchThat (is_reification_of reified_inner_loop_hd_gen inner_loop_hd)
+         As reified_inner_loop_hd_gen_correct.
+  Proof. Time cache_reify (). Time Qed.
+  Hint Extern 1 (_ = _) => apply_cached_reification inner_loop_hd (proj1 reified_inner_loop_hd_gen_correct) : reify_cache_gen.
+  Hint Immediate (proj2 reified_inner_loop_hd_gen_correct) : wf_gen_cache.
+  Hint Rewrite (proj1 reified_inner_loop_hd_gen_correct) : interp_gen_cache.
+  Local Opaque reified_inner_loop_hd_gen. (* needed for making [autorewrite] not take a very long time *)
+
+  (* this got too slow after generalizing d in jumpdivstep
+
+  Derive reified_jump_divstep_gen
+         SuchThat (is_reification_of reified_jump_divstep_gen jump_divstep)
+         As reified_jump_divstep_gen_correct.
+  Proof. Time cache_reify (). Time Qed.
+  Hint Extern 1 (_ = _) => apply_cached_reification jump_divstep (proj1 reified_jump_divstep_gen_correct) : reify_cache_gen.
+  Hint Immediate (proj2 reified_jump_divstep_gen_correct) : wf_gen_cache.
+  Hint Rewrite (proj1 reified_jump_divstep_gen_correct) : interp_gen_cache.
+  Local Opaque reified_jump_divstep_gen. (* needed for making [autorewrite] not take a very long time *)
+
+  Derive reified_jump_divstep_hd_gen
+         SuchThat (is_reification_of reified_jump_divstep_hd_gen jump_divstep_hd)
+         As reified_jump_divstep_hd_gen_correct.
+  Proof. Time cache_reify (). Time Qed.
+  Hint Extern 1 (_ = _) => apply_cached_reification jump_divstep_hd (proj1 reified_jump_divstep_hd_gen_correct) : reify_cache_gen.
+  Hint Immediate (proj2 reified_jump_divstep_hd_gen_correct) : wf_gen_cache.
+  Hint Rewrite (proj1 reified_jump_divstep_hd_gen_correct) : interp_gen_cache.
+  Local Opaque reified_jump_divstep_hd_gen. (* needed for making [autorewrite] not take a very long time *)
+
+  *)
 
   Derive reified_divstep_gen
          SuchThat (is_reification_of reified_divstep_gen divstep)
@@ -41,23 +120,75 @@ Module Export WordByWordMontgomeryInversion.
   Hint Rewrite (proj1 reified_divstep_gen_correct) : interp_gen_cache.
   Local Opaque reified_divstep_gen. (* needed for making [autorewrite] not take a very long time *)
 
-  Derive reified_msat_gen
-         SuchThat (is_reification_of reified_msat_gen msat)
-         As reified_msat_gen_correct.
-  Proof.
-    Time cache_reify ().
-    Time Qed.
-  Hint Extern 1 (_ = _) => apply_cached_reification msat (proj1 reified_msat_gen_correct) : reify_cache_gen.
-  Hint Immediate (proj2 reified_msat_gen_correct) : wf_gen_cache.
-  Hint Rewrite (proj1 reified_msat_gen_correct) : interp_gen_cache.
-  Local Opaque reified_msat_gen. (* needed for making [autorewrite] not take a very long time *)
+End WordByWordMontgomery.
 
-  Derive reified_eval_twos_complement_gen
-         SuchThat (is_reification_of reified_eval_twos_complement_gen eval_twos_complement)
-         As reified_eval_twos_complement_gen_correct.
+Module Export UnsaturatedSolinas.
+  Import Definitions.UnsaturatedSolinas.
+
+  Derive reified_update_fg_gen
+         SuchThat (is_reification_of reified_update_fg_gen update_fg)
+         As reified_update_fg_gen_correct.
   Proof. Time cache_reify (). Time Qed.
-  Hint Extern 1 (_ = _) => apply_cached_reification eval_twos_complement (proj1 reified_eval_twos_complement_gen_correct) : reify_cache_gen.
-  Hint Immediate (proj2 reified_eval_twos_complement_gen_correct) : wf_gen_cache.
-  Hint Rewrite (proj1 reified_eval_twos_complement_gen_correct) : interp_gen_cache.
-  Local Opaque reified_eval_twos_complement_gen. (* needed for making [autorewrite] not take a very long time *)
-End WordByWordMontgomeryInversion.
+  Hint Extern 1 (_ = _) => apply_cached_reification update_fg (proj1 reified_update_fg_gen_correct) : reify_cache_gen.
+  Hint Immediate (proj2 reified_update_fg_gen_correct) : wf_gen_cache.
+  Hint Rewrite (proj1 reified_update_fg_gen_correct) : interp_gen_cache.
+  Local Opaque reified_update_fg_gen. (* needed for making [autorewrite] not take a very long time *)
+
+  Derive reified_update_vr_gen
+         SuchThat (is_reification_of reified_update_vr_gen update_vr)
+         As reified_update_vr_gen_correct.
+  Proof. Time cache_reify (). Time Qed.
+  Hint Extern 1 (_ = _) => apply_cached_reification update_vr (proj1 reified_update_vr_gen_correct) : reify_cache_gen.
+  Hint Immediate (proj2 reified_update_vr_gen_correct) : wf_gen_cache.
+  Hint Rewrite (proj1 reified_update_vr_gen_correct) : interp_gen_cache.
+  Local Opaque reified_update_vr_gen. (* needed for making [autorewrite] not take a very long time *)
+
+  Derive reified_inner_loop_gen
+         SuchThat (is_reification_of reified_inner_loop_gen inner_loop)
+         As reified_inner_loop_gen_correct.
+  Proof. Time cache_reify (). Time Qed.
+  Hint Extern 1 (_ = _) => apply_cached_reification inner_loop (proj1 reified_inner_loop_gen_correct) : reify_cache_gen.
+  Hint Immediate (proj2 reified_inner_loop_gen_correct) : wf_gen_cache.
+  Hint Rewrite (proj1 reified_inner_loop_gen_correct) : interp_gen_cache.
+  Local Opaque reified_inner_loop_gen. (* needed for making [autorewrite] not take a very long time *)
+
+  Derive reified_inner_loop_hd_gen
+         SuchThat (is_reification_of reified_inner_loop_hd_gen inner_loop_hd)
+         As reified_inner_loop_hd_gen_correct.
+  Proof. Time cache_reify (). Time Qed.
+  Hint Extern 1 (_ = _) => apply_cached_reification inner_loop_hd (proj1 reified_inner_loop_hd_gen_correct) : reify_cache_gen.
+  Hint Immediate (proj2 reified_inner_loop_hd_gen_correct) : wf_gen_cache.
+  Hint Rewrite (proj1 reified_inner_loop_hd_gen_correct) : interp_gen_cache.
+  Local Opaque reified_inner_loop_hd_gen. (* needed for making [autorewrite] not take a very long time *)
+
+  (* this got too slow after generalizing d in jumpdivstep
+
+  Derive reified_jump_divstep_gen
+         SuchThat (is_reification_of reified_jump_divstep_gen jump_divstep)
+         As reified_jump_divstep_gen_correct.
+  Proof. Time cache_reify (). Time Qed.
+  Hint Extern 1 (_ = _) => apply_cached_reification jump_divstep (proj1 reified_jump_divstep_gen_correct) : reify_cache_gen.
+  Hint Immediate (proj2 reified_jump_divstep_gen_correct) : wf_gen_cache.
+  Hint Rewrite (proj1 reified_jump_divstep_gen_correct) : interp_gen_cache.
+  Local Opaque reified_jump_divstep_gen. (* needed for making [autorewrite] not take a very long time *)
+
+  Derive reified_jump_divstep_hd_gen
+         SuchThat (is_reification_of reified_jump_divstep_hd_gen jump_divstep_hd)
+         As reified_jump_divstep_hd_gen_correct.
+  Proof. Time cache_reify (). Time Qed.
+  Hint Extern 1 (_ = _) => apply_cached_reification jump_divstep_hd (proj1 reified_jump_divstep_hd_gen_correct) : reify_cache_gen.
+  Hint Immediate (proj2 reified_jump_divstep_hd_gen_correct) : wf_gen_cache.
+  Hint Rewrite (proj1 reified_jump_divstep_hd_gen_correct) : interp_gen_cache.
+  Local Opaque reified_jump_divstep_hd_gen. (* needed for making [autorewrite] not take a very long time *)
+
+  *)
+
+  Derive reified_divstep_gen
+         SuchThat (is_reification_of reified_divstep_gen divstep)
+         As reified_divstep_gen_correct.
+  Proof. Time cache_reify (). Time Qed.
+  Hint Extern 1 (_ = _) => apply_cached_reification divstep (proj1 reified_divstep_gen_correct) : reify_cache_gen.
+  Hint Immediate (proj2 reified_divstep_gen_correct) : wf_gen_cache.
+  Hint Rewrite (proj1 reified_divstep_gen_correct) : interp_gen_cache.
+  Local Opaque reified_divstep_gen. (* needed for making [autorewrite] not take a very long time *)
+End UnsaturatedSolinas.
