src/PushButtonSynthesis/WordByWordMontgomery.v
@@ -41,7 +41,7 @@ Require Import Crypto.Arithmetic.Freeze.
 Require Import Crypto.Arithmetic.Partition.
 Require Import Crypto.Arithmetic.WordByWordMontgomery.
 Require Import Crypto.Arithmetic.UniformWeight.
-Require Import Crypto.Arithmetic.BYInv.
+Require Import Crypto.Arithmetic.BYInv.Definitions.
 Require Import Crypto.BoundsPipeline.
 Require Import Crypto.COperationSpecifications.
 Require Import Crypto.PushButtonSynthesis.ReificationCache.
@@ -68,7 +68,7 @@ Import Associational Positional.
 Import Arithmetic.WordByWordMontgomery.WordByWordMontgomery.
 
 Import WordByWordMontgomeryReificationCache.WordByWordMontgomery.
-Import BYInversionReificationCache.WordByWordMontgomeryInversion.
+Import BYInversionReificationCache.WordByWordMontgomery.
 
 Local Coercion Z.of_nat : nat >-> Z.
 Local Coercion QArith_base.inject_Z : Z >-> Q.
@@ -125,22 +125,21 @@ Section __.
   Definition s := 2^Z.log2_up m.
   Definition c := s - m.
   Definition n : nat := Z.to_nat (Qceiling (Z.log2_up s / machine_wordsize)).
-  Definition sat_limbs := (n + 1)%nat.   (* to represent m in twos complement we might need another bit *)
+  Definition m_bits := Z.log2 m + 1.
+  Definition sat_limbs := Z.to_nat (((m_bits - 1) / machine_wordsize) + 2). (* the two extra bits are for sign and to store the first addition in divstep which might be twice as big as m *)
+  Definition sat_upper_bound := 2 ^ (sat_limbs * machine_wordsize) - 1.
+  Definition word_sat_mul_limbs := (sat_limbs + 1)%nat. (* to store the result of a multiplication of signed multilimb with a word *)
   Definition r := 2^machine_wordsize.
   Definition r' := Z.modinv r m.
   Definition m' := Z.modinv (-m) r.
   Definition n_bytes := bytes_n s.
 
-  Definition divstep_precompmod :=
-    let bits := (Z.log2 m) + 1 in
-    let i := if bits <? 46 then (49 * bits + 80) / 17 else (49 * bits + 57) / 17 in
-    let k := (m + 1) / 2 in
-    (Z.modexp k i m).
-
   Definition prime_upperbound_list : list Z
     := Partition.partition (uweight machine_wordsize) n (s-1).
   Definition prime_bytes_upperbound_list : list Z
     := Partition.partition (weight 8 1) n_bytes (s-1).
+  Definition saturated_bytes_list : list Z
+    := Partition.partition (weight 8 1) n_bytes sat_upper_bound.
   Definition upperbounds : list Z := prime_upperbound_list.
   Definition prime_bound : ZRange.type.interp (base.type.Z)
     := r[0~>m-1]%zrange.
@@ -150,10 +149,15 @@ Section __.
     := List.map (fun v => Some r[0 ~> v]%zrange) prime_upperbound_list.
   Definition prime_bytes_bounds : list (ZRange.type.option.interp (base.type.Z))
     := List.map (fun v => Some r[0 ~> v]%zrange) prime_bytes_upperbound_list.
+  Definition saturated_bytes_bounds : ZRange.type.option.interp (base.type.list (base.type.Z))
+    := Some (List.map (fun v => Some r[0 ~> v]%zrange) saturated_bytes_list).
   Local Notation word_bound := (word_bound machine_wordsize).
   Local Notation saturated_bounds := (saturated_bounds n machine_wordsize).
   Local Notation larger_saturated_bounds := (Primitives.saturated_bounds sat_limbs machine_wordsize).
 
+  Local Notation divstep_precompmod := (divstep_precompmod machine_wordsize n m).
+  Local Notation jumpdivstep_precompmod := (jumpdivstep_precompmod machine_wordsize n m).
+  Local Notation jumpdivstep_precompmod_hd := (jumpdivstep_precompmod_hd machine_wordsize n m).
 
   Definition divstep_input :=
     (Some r[0~>2^machine_wordsize-1],
@@ -167,6 +171,55 @@ Section __.
      Some (repeat (Some r[0 ~> 2^machine_wordsize-1]) sat_limbs),
      Some (repeat (Some r[0 ~> 2^machine_wordsize-1]) sat_limbs),
      Some (repeat (Some r[0 ~> 2^machine_wordsize-1]) n),
+     Some (repeat (Some r[0 ~> 2^machine_wordsize-1]) n))%zrange.
+
+  (* these are for jumpdivstep, if it could be reified (currently too slow) *)
+  (* Definition jump_divstep_input := *)
+  (*   (Some (repeat (Some r[0 ~> 2^machine_wordsize-1]) sat_limbs), *)
+  (*    (Some (repeat (Some r[0 ~> 2^machine_wordsize-1]) sat_limbs), *)
+  (*     (Some (repeat (Some r[0 ~> 2^machine_wordsize-1]) n), *)
+  (*      (Some (repeat (Some r[0 ~> 2^machine_wordsize-1]) n), tt))))%zrange. *)
+
+  (* Definition jump_divstep_output := *)
+  (*   (Some (repeat (Some r[0 ~> 2^machine_wordsize-1]) sat_limbs), *)
+  (*    Some (repeat (Some r[0 ~> 2^machine_wordsize-1]) sat_limbs), *)
+  (*    Some (repeat (Some r[0 ~> 2^machine_wordsize-1]) n), *)
+  (*    Some (repeat (Some r[0 ~> 2^machine_wordsize-1]) n))%zrange. *)
+
+  Definition inner_loop_input :=
+    (Some r[0~>2^machine_wordsize-1],
+      (Some (repeat (Some r[0 ~> 2^machine_wordsize-1]) sat_limbs),
+        (Some (repeat (Some r[0 ~> 2^machine_wordsize-1]) sat_limbs), tt)))%zrange.
+
+  Definition inner_loop_output :=
+    (Some r[0 ~> 2^machine_wordsize-1],
+     Some r[0 ~> 2^machine_wordsize-1],
+     Some r[0 ~> 2^machine_wordsize-1],
+     Some r[0 ~> 2^machine_wordsize-1],
+     Some r[0 ~> 2^machine_wordsize-1])%zrange.
+
+  Definition update_fg_input :=
+    (Some (repeat (Some r[0 ~> 2^machine_wordsize-1]) sat_limbs),
+      (Some (repeat (Some r[0 ~> 2^machine_wordsize-1]) sat_limbs),
+        (Some r[0 ~> 2^machine_wordsize-1],
+          (Some r[0 ~> 2^machine_wordsize-1],
+            (Some r[0 ~> 2^machine_wordsize-1],
+              (Some r[0 ~> 2^machine_wordsize-1], tt))))))%zrange.
+
+  Definition update_fg_output :=
+    (Some (repeat (Some r[0 ~> 2^machine_wordsize-1]) sat_limbs),
+     Some (repeat (Some r[0 ~> 2^machine_wordsize-1]) sat_limbs))%zrange.
+
+  Definition update_vr_input :=
+    (Some (repeat (Some r[0 ~> 2^machine_wordsize-1]) n),
+      (Some (repeat (Some r[0 ~> 2^machine_wordsize-1]) n),
+        (Some r[0 ~> 2^machine_wordsize-1],
+          (Some r[0 ~> 2^machine_wordsize-1],
+            (Some r[0 ~> 2^machine_wordsize-1],
+              (Some r[0 ~> 2^machine_wordsize-1], tt))))))%zrange.
+
+  Definition update_vr_output :=
+    (Some (repeat (Some r[0 ~> 2^machine_wordsize-1]) n),
      Some (repeat (Some r[0 ~> 2^machine_wordsize-1]) n))%zrange.
 
   (* We include [0], so that even after bounds relaxation, we can
@@ -193,7 +246,6 @@ Section __.
   Global Instance non_montgomery_domain_bounds_typedef : typedef (t:=base.type.list base.type.Z) (Some non_montgomery_domain_bounds)
     := { name := "non_montgomery_domain_field_element"
          ; description name := (text_before_type_name ++ name ++ " is a field element NOT in the Montgomery domain.")%string }.
-
 
   Local Instance no_select_size : no_select_size_opt := no_select_size_of_no_select machine_wordsize.
   Local Instance split_mul_to : split_mul_to_opt := split_mul_to_of_should_split_mul machine_wordsize possible_values.
@@ -289,7 +341,7 @@ Section __.
                             (CorrectnessStringification.dyn_context.cons
                                (Z.log2 m) "⌊log2 m⌋"
                                (CorrectnessStringification.dyn_context.cons
-                                  (@eval_twos_complement machine_wordsize n) "twos_complement_eval"
+                                  (tc_eval machine_wordsize n) "twos_complement_eval"
                                   CorrectnessStringification.dyn_context.nil)))))))%string)
          (only parsing).
   Local Notation "'docstring_with_summary_from_lemma!' prefix summary correctness"
@@ -637,7 +689,7 @@ Section __.
          true (* subst01 *)
          None (* fancy *)
          possible_values
-         (reified_msat_gen
+         (reified_partition_gen
             @ GallinaReify.Reify (machine_wordsize:Z) @ GallinaReify.Reify sat_limbs @ GallinaReify.Reify m)
          tt
          (Some larger_bounds).
@@ -657,8 +709,8 @@ Section __.
          true (* subst01 *)
          None (* fancy *)
          possible_values
-         (reified_encode_gen
-            @ GallinaReify.Reify (machine_wordsize:Z) @ GallinaReify.Reify n @ GallinaReify.Reify m @ GallinaReify.Reify m' @ GallinaReify.Reify divstep_precompmod)
+         (reified_partition_gen
+            @ GallinaReify.Reify (machine_wordsize:Z) @ GallinaReify.Reify n @ GallinaReify.Reify divstep_precompmod)
          tt
          (Some bounds).
 
@@ -678,7 +730,10 @@ Section __.
          None (* fancy *)
          possible_values
          (reified_divstep_gen
-            @ GallinaReify.Reify (machine_wordsize:Z) @ GallinaReify.Reify sat_limbs @ GallinaReify.Reify n @ GallinaReify.Reify m)
+            @ GallinaReify.Reify (machine_wordsize:Z)
+            @ GallinaReify.Reify n
+            @ GallinaReify.Reify sat_limbs
+            @ GallinaReify.Reify m)
          (divstep_input)
          (divstep_output).
 
@@ -691,6 +746,210 @@ Section __.
              prefix
              (fun fname : string => [text_before_function_name ++ fname ++ " computes a divstep."]%string)
              (divstep_correct machine_wordsize n m valid from_montgomery_res)).
+
+  Definition inner_loop
+    := Pipeline.BoundsPipeline
+         false (* subst01 *)
+         None (* fancy *)
+         possible_values
+         (reified_inner_loop_gen
+            @ GallinaReify.Reify (machine_wordsize:Z))
+         (inner_loop_input)
+         (inner_loop_output).
+
+  Definition sinner_loop (prefix : string)
+    : string * (Pipeline.ErrorT (Pipeline.ExtendedSynthesisResult _))
+    := Eval cbv beta in
+        FromPipelineToString!
+          machine_wordsize prefix "inner_loop" inner_loop
+          (docstring_with_summary_from_lemma!
+             prefix
+             (fun fname : string => [text_before_function_name ++ fname ++ " computes a inner_loop."]%string)
+             (forall v, valid v)).
+
+  Definition inner_loop_hd
+    := Pipeline.BoundsPipeline
+         false (* subst01 *)
+         None (* fancy *)
+         possible_values
+         (reified_inner_loop_hd_gen
+            @ GallinaReify.Reify (machine_wordsize:Z))
+         (inner_loop_input)
+         (inner_loop_output).
+
+  Definition sinner_loop_hd (prefix : string)
+    : string * (Pipeline.ErrorT (Pipeline.ExtendedSynthesisResult _))
+    := Eval cbv beta in
+        FromPipelineToString!
+          machine_wordsize prefix "inner_loop_hd" inner_loop_hd
+          (docstring_with_summary_from_lemma!
+             prefix
+             (fun fname : string => [text_before_function_name ++ fname ++ " computes a inner_loop_hd."]%string)
+             (forall v, valid v)).
+
+  Definition update_fg
+    := Pipeline.BoundsPipeline
+         false (* subst01 *)
+         None (* fancy *)
+         possible_values
+         (reified_update_fg_gen
+            @ GallinaReify.Reify (machine_wordsize:Z)
+            @ GallinaReify.Reify sat_limbs
+            @ GallinaReify.Reify word_sat_mul_limbs)
+         (update_fg_input)
+         (update_fg_output).
+
+  Definition supdate_fg (prefix : string)
+    : string * (Pipeline.ErrorT (Pipeline.ExtendedSynthesisResult _))
+    := Eval cbv beta in
+        FromPipelineToString!
+          machine_wordsize prefix "update_fg" update_fg
+          (docstring_with_summary_from_lemma!
+             prefix
+             (fun fname : string => [text_before_function_name ++ fname ++ " computes a update_fg."]%string)
+             (forall v, valid v)).
+
+  Definition update_vr
+    := Pipeline.BoundsPipeline
+         false (* subst01 *)
+         None (* fancy *)
+         possible_values
+         (reified_update_vr_gen
+            @ GallinaReify.Reify (machine_wordsize:Z)
+            @ GallinaReify.Reify n
+            @ GallinaReify.Reify m
+            @ GallinaReify.Reify m')
+         (update_vr_input)
+         (update_vr_output).
+
+  Definition supdate_vr (prefix : string)
+    : string * (Pipeline.ErrorT (Pipeline.ExtendedSynthesisResult _))
+    := Eval cbv beta in
+        FromPipelineToString!
+          machine_wordsize prefix "update_vr" update_vr
+          (docstring_with_summary_from_lemma!
+             prefix
+             (fun fname : string => [text_before_function_name ++ fname ++ " computes a update_vr."]%string)
+             (forall v, valid v)).
+
+  Definition sat_from_bytes
+    := Pipeline.BoundsPipeline
+         false (* subst01 *)
+         None (* fancy *)
+         possible_values_with_bytes
+         (reified_from_bytes_gen
+            @ GallinaReify.Reify (machine_wordsize:Z) @ GallinaReify.Reify 1 @ GallinaReify.Reify sat_upper_bound @ GallinaReify.Reify sat_limbs)
+         (saturated_bytes_bounds, tt)
+         (Some larger_bounds).
+
+  Definition ssat_from_bytes (prefix : string)
+    : string * (Pipeline.ErrorT (Pipeline.ExtendedSynthesisResult _))
+    := Eval cbv beta in
+        FromPipelineToString!
+          machine_wordsize prefix "sat_from_bytes" sat_from_bytes
+          (docstring_with_summary_from_lemma!
+             prefix
+             (fun fname : string => ["The function " ++ fname ++ " deserializes a field element NOT in the Montgomery domain from bytes in little-endian order."]%string)
+             (forall v, valid v)).
+             (* (from_bytes_correct machine_wordsize n n_bytes m valid bytes_valid)). *)
+
+  Definition jumpdivstep_precomp
+    := Pipeline.BoundsPipeline
+         true (* subst01 *)
+         None (* fancy *)
+         possible_values
+         (reified_partition_gen
+            @ GallinaReify.Reify (machine_wordsize:Z)
+            @ GallinaReify.Reify n
+            @ GallinaReify.Reify jumpdivstep_precompmod)
+         tt
+         (Some bounds).
+
+  Definition sjumpdivstep_precomp (prefix : string)
+    : string * (Pipeline.ErrorT (Pipeline.ExtendedSynthesisResult _))
+    := Eval cbv beta in
+        FromPipelineToString!
+          machine_wordsize prefix "jumpdivstep_precomp" jumpdivstep_precomp
+          (docstring_with_summary_from_lemma!
+             prefix
+             (fun fname => ["The function " ++ fname ++ " returns the precomputed value for the jump-version of Bernstein-Yang-inversion (in montgomery form)."]%string)
+             (divstep_precomp_correct machine_wordsize n m valid from_montgomery_res)).
+
+  Definition jumpdivstep_precomp_hd
+    := Pipeline.BoundsPipeline
+         true (* subst01 *)
+         None (* fancy *)
+         possible_values
+         (reified_partition_gen
+            @ GallinaReify.Reify (machine_wordsize:Z)
+            @ GallinaReify.Reify n
+            @ GallinaReify.Reify jumpdivstep_precompmod_hd)
+         tt
+         (Some bounds).
+
+  Definition sjumpdivstep_precomp_hd (prefix : string)
+    : string * (Pipeline.ErrorT (Pipeline.ExtendedSynthesisResult _))
+    := Eval cbv beta in
+        FromPipelineToString!
+          machine_wordsize prefix "jumpdivstep_precomp_hd" jumpdivstep_precomp_hd
+          (docstring_with_summary_from_lemma!
+             prefix
+             (fun fname => ["The function " ++ fname ++ " returns the precomputed value for the (half-delta) jump-version of Bernstein-Yang-inversion (in montgomery form)."]%string)
+             (divstep_precomp_correct machine_wordsize n m valid from_montgomery_res)).
+
+  (* not currently viable (see BYInversionReificationCache)
+  Definition jump_divstep
+    := Pipeline.BoundsPipeline
+         false (* subst01 *)
+         None (* fancy *)
+         possible_values
+         (reified_jump_divstep_gen
+            @ GallinaReify.Reify (machine_wordsize:Z)
+            @ GallinaReify.Reify n
+            @ GallinaReify.Reify sat_limbs
+            @ GallinaReify.Reify word_sat_mul_limbs
+            @ GallinaReify.Reify m
+            @ GallinaReify.Reify m')
+         loop_input
+         loop_output.
+
+  Definition sjump_divstep (prefix : string)
+    : string * (Pipeline.ErrorT (Pipeline.ExtendedSynthesisResult _))
+    := Eval cbv beta in
+        FromPipelineToString!
+          machine_wordsize prefix "jump_divstep" jump_divstep
+          (docstring_with_summary_from_lemma!
+             prefix
+             (fun fname : string => ["The function " ++ fname ++ " computes the body of the outer loop in BY-inversion (jumpdivstep version)."]%string)
+             (forall v, valid v)).
+             (* (jump_divstep_correct weightu sat_limbs)). *)
+
+  Definition jump_divstep_hd
+    := Pipeline.BoundsPipeline
+         false (* subst01 *)
+         None (* fancy *)
+         possible_values
+         (reified_jump_divstep_hd_gen
+            @ GallinaReify.Reify (machine_wordsize:Z)
+            @ GallinaReify.Reify n
+            @ GallinaReify.Reify sat_limbs
+            @ GallinaReify.Reify word_sat_mul_limbs
+            @ GallinaReify.Reify m
+            @ GallinaReify.Reify m')
+         loop_input
+         loop_output.
+
+  Definition sjump_divstep_hd (prefix : string)
+    : string * (Pipeline.ErrorT (Pipeline.ExtendedSynthesisResult _))
+    := Eval cbv beta in
+        FromPipelineToString!
+          machine_wordsize prefix "jump_divstep_hd" jump_divstep_hd
+          (docstring_with_summary_from_lemma!
+             prefix
+             (fun fname : string => ["The function " ++ fname ++ " computes the body of the outer loop in BY-inversion (jumpdivstep version)."]%string)
+             (forall v, valid v)).
+             (* (jump_divstep_hd_correct weightu sat_limbs)). *)
+   *)
 
   Lemma bounded_by_of_valid x
         (H : valid x)
@@ -1112,7 +1371,16 @@ Section __.
             ("one", wrap_s sone);
             ("msat", wrap_s smsat);
             ("divstep_precomp", wrap_s sdivstep_precomp);
-            ("divstep", wrap_s sdivstep)].
+            ("divstep", wrap_s sdivstep);
+            ("sat_from_bytes", wrap_s ssat_from_bytes);
+            ("jumpdivstep_precomp", wrap_s sjumpdivstep_precomp);
+            ("jumpdivstep_precomp_hd", wrap_s sjumpdivstep_precomp_hd);
+            ("inner_loop", wrap_s sinner_loop);
+            ("inner_loop_hd", wrap_s sinner_loop_hd);
+            ("update_fg", wrap_s supdate_fg);
+            ("update_vr", wrap_s supdate_vr)].
+            (* ("jump_divstep", wrap_s sjump_divstep); *)
+            (* ("jump_divstep_hd", wrap_s sjump_divstep_hd)]. *)
 
     Definition valid_names : string := Eval compute in String.concat ", " (List.map (@fst _ _) known_functions).
 
