src/Util/ZUtil/OnesAt.v
@@ -1,0 +1,21 @@
+Require Import Coq.Bool.Bool.
+Require Import Coq.ZArith.ZArith.
+
+Require Import Crypto.Util.ZUtil.Definitions.
+Require Import Crypto.Util.ZUtil.Testbit.
+
+Require Import Crypto.Util.ZUtil.Tactics.SolveTestbit.
+
+Local Open Scope Z_scope.
+
+Module Z.
+  Lemma ones_at_spec_full m k i
+        (Hk : 0 <= k) :
+    Z.testbit (Z.ones_at m k) i = if (i <? 0) then false else (m <=? i) && (i <? m + k).
+  Proof. unfold Z.ones_at; Z.solve_testbit. Qed.
+
+  Hint Rewrite ones_at_spec_full : testbit_rewrite.
+
+  Lemma ones_at_0 m : Z.ones_at m 0 = 0.
+  Proof. Z.solve_using_testbit. Qed.
+End Z.
