src/Util/ZUtil/TruncatingShiftl.v
@@ -13,7 +13,7 @@ Module Z.
   Proof. reflexivity. Qed.
 
   Lemma truncating_shiftl_correct_land_ones bw x y
-  : Z.truncating_shiftl bw x y = (x << y) &' 
+  : Z.truncating_shiftl bw x y = (x << y) &'
       Z.ones ltac:(match eval hnf in (1 mod 0) with | 0 => exact (Z.max 0 bw) | _ => exact bw end).
   Proof.
     rewrite truncating_shiftl_correct.
@@ -37,12 +37,13 @@ Module Z.
   Proof.
     unfold Definitions.Z.truncating_shiftl. rewrite Z.shiftl_mul_pow2 by lia.
     replace (2^b) with (2 * 2^(b-1)) by (rewrite Pow.Z.pow_mul_base, Z.sub_simpl_r; lia).
-    rewrite Zmult_mod_distr_r; ring. Qed.
+    rewrite Zmult_mod_distr_r; ring.
+  Qed.
 
   Lemma truncating_shiftl_testbit_spec_full m a k i :
     Z.testbit (Z.truncating_shiftl m a k) i
     = if (i <? 0) then false else if (orb (i <? m) ((1 mod 0 =? 1) && (m <? 0))) then Z.testbit a (i - k) else false.
-  Proof. unfold Z.truncating_shiftl. Z.solve_testbit. Qed.
+  Proof. unfold Z.truncating_shiftl. Z.solve_testbit; cbn in *; lia. Qed.
 
   Hint Rewrite truncating_shiftl_testbit_spec_full : testbit_rewrite.
 
@@ -52,6 +53,7 @@ Module Z.
     Z.truncating_shiftl m (Z.truncating_shiftl m a p) q
     = Z.truncating_shiftl m a (p + q).
   Proof. Z.solve_using_testbit. Qed.
+
   Lemma truncating_shiftl0 m k :
     Z.truncating_shiftl m 0 k = 0.
   Proof. Z.solve_using_testbit. Qed.
@@ -61,10 +63,9 @@ Module Z.
     = (Z.truncating_shiftl m a k) |' (Z.truncating_shiftl m b k).
   Proof. Z.solve_using_testbit. Qed.
 
-  (* (* not compatible with x mod 0 = x *)
-  Lemma truncating_shiftl_large m a k (Hk : k >= m) :
+  Lemma truncating_shiftl_large m a k (Hm : 0 <= m) (Hk : k >= m) :
     Z.truncating_shiftl m a k = 0.
-  Proof. Z.solve_using_testbit. Qed. *)
+  Proof. Z.solve_using_testbit. Qed.
 
   Lemma truncating_shiftl_range m a k (Hm : 0 <= m) :
     0 <= Z.truncating_shiftl m a k < 2 ^ m.
